running time proof

Cslib/Languages/Boole/examples/MergeSort/mergeSort.lean
@@ -1,6 +1,10 @@
 import Mathlib.Data.Nat.Basic
 import Init.Data.Option.Coe
 import Mathlib.Order.Lattice
+import Mathlib.Data.List.Sort
+import Mathlib.Tactic.Ring.Basic
+import Mathlib.Tactic.Ring.RingNF
+import Mathlib.Data.Nat.Log
 
 set_option tactic.hygienic false
 
@@ -75,9 +79,151 @@ termination_by xs.length decreasing_by (
 
 #check mergeSort
 #eval merge [1,2,3,10] [4,5]
-#eval! mergeSort [4,2,3,5]
+#eval! mergeSort [4,2,3,]
 
 #check merge.go.induct
 #check mergeSort.induct
+
+open List
+
+@[simp, grind] def IsSorted (l : List ℕ) : Prop := Sorted (· ≤ ·) l
+@[simp, grind] def MinOfList (x : ℕ) (l : List ℕ) : Prop := ∀ b ∈ l, x ≤ b
+
+theorem mem_either_merge (xs ys : List ℕ) (z : ℕ)
+  (hz : z ∈ (merge xs ys).val) : z ∈ xs ∨ z ∈ ys := by
+  rw [merge] at hz
+  fun_induction merge.go <;>
+  all_goals (try (simp only [not_mem_nil, false_or];assumption))
+  all_goals (simp only [Bind.bind, tick, val_bind, mem_cons] at hz;cases hz;all_goals (aesop))
+
+
+theorem min_all_merge (x : ℕ) (xs ys : List ℕ)
+(hxs : MinOfList x xs) (hys : MinOfList x ys) : MinOfList x (merge xs ys).val := by
+  simp_all only [MinOfList]
+  intro a ha
+  apply mem_either_merge at ha
+  grind
+
+theorem sorted_merge (l1 l2 : List ℕ) (hxs : IsSorted l1)
+  (hys : IsSorted l2) : IsSorted ((merge l1 l2).val) := by
+  fun_induction merge.go l1 l2 <;> all_goals (first| simpa [merge,merge.go,tick]|
+    simp only [IsSorted, merge, merge.go, h, ↓reduceIte, Bind.bind, tick, val_bind, sorted_cons]
+    simp [merge] at ih1
+    simp_all only [IsSorted, sorted_cons, implies_true, forall_const, and_true]
+    apply min_all_merge <;> all_goals grind
+  )
+
+theorem MSMCorrect (xs : List ℕ) : IsSorted (mergeSort xs).val := by
+  fun_induction mergeSort xs
+  · obtain h | h : x = [] ∨ ∃a, x = [a] := by
+      by_cases x.length = 0
+      · aesop
+      · right
+        have: x.length = 1 := by omega
+        exact List.length_eq_one_iff.mp this
+    · subst h
+      simp only [IsSorted]
+      exact sorted_nil
+    · obtain ⟨a,ha⟩ := h
+      rw [ha]
+      exact sorted_singleton a
+  · simp only [Bind.bind, val_bind]
+    apply sorted_merge
+    · exact ih2
+    · exact ih1
+
+@[simp] theorem merge_cost (xs ys : List ℕ) : (merge xs ys).cost = xs.length + ys.length := by
+  simp only [merge]
+  fun_induction merge.go <;>
+  all_goals(simp_all only [length_cons, Bind.bind, tick, cost_of_bind]; all_goals (grind))
+
+@[simp] theorem merge_val_length_eq_sum (xs ys : List ℕ) :
+  (merge xs ys).val.length = xs.length + ys.length := by
+  rw [merge]
+  fun_induction merge.go <;> all_goals (simp_all only
+  [length_cons, Bind.bind, tick, val_bind]; grind [Bind.bind,tick,val_bind])
+
+
+@[simp] theorem mergeSort_same_length (xs : List ℕ) : (mergeSort xs).val.length = xs.length:= by
+  fun_induction mergeSort <;> all_goals (try simp_all only [pure,not_lt, Bind.bind, val_bind])
+  grind [merge_val_length_eq_sum]
+
+#check Bind.bind
+#check Pure.pure
+
+theorem mergeSort_cost_recurrence (xs : List ℕ) (h : 2 ≤ xs.length) :
+  (mergeSort xs).cost = (mergeSort (xs.take (xs.length / 2))).cost +
+                        (mergeSort (xs.drop (xs.length / 2))).cost +
+                        xs.length := by
+  conv =>
+    left
+    unfold mergeSort
+  split_ifs with h1
+  · omega
+  · dsimp [Bind.bind,cost_of_bind]
+    ring_nf
+    simp only [merge_cost, Nat.add_left_cancel_iff]
+    repeat rw [mergeSort_same_length]
+    simp only [length_take, length_drop]
+    omega
+
+def MS_REC : ℕ → ℕ
+| 0 => 0
+| x+1 =>
+  if x = 0 then 0
+  else
+    let n := x+1
+    MS_REC (n/2) + MS_REC ((n-1)/2 + 1) + n
+termination_by x => x decreasing_by all_goals omega
+
+#eval! mergeSort [4,1,3,4,5,6]
+#eval! MS_REC 6
+
+
+theorem mergeSort_cost_eq_MS_REC (xs : List ℕ) :
+  (mergeSort xs).cost = MS_REC xs.length := by
+  fun_induction mergeSort
+  · simp only [cost_of_pure]
+    unfold MS_REC
+    simp only [Nat.add_one_sub_one]
+    grind
+  · simp_all only [not_lt, Bind.bind, cost_of_bind, merge_cost, mergeSort_same_length]
+    conv =>
+      right
+      unfold MS_REC
+    simp only [Nat.add_one_sub_one]
+    split <;> all_goals (grind)
+
+
+def MS_REC_SIMP : ℕ → ℕ
+| 0 => 0
+| x+1 =>
+  if x = 0 then 0
+  else
+    let n := x+1
+    2*MS_REC_SIMP (n/2) + n
+
+theorem MS_REC_SIMP_EQ (n : ℕ) :   (MS_REC (2^n))= (MS_REC_SIMP (2^n))  := by
+  induction' n  with n ih
+  · unfold MS_REC_SIMP MS_REC
+    simp only [↓reduceIte]
+  · unfold MS_REC_SIMP MS_REC
+    split <;> all_goals grind
+
+
+theorem MS_REC_SIMP_EQ_CLOSED (n : ℕ) : MS_REC_SIMP (2^n) = 2^n * n := by
+  induction' n  with n ih
+  · unfold MS_REC_SIMP
+    aesop
+  · unfold MS_REC_SIMP
+    grind
+
+-- The cost is written assuming the length of the list is a power of two (for simplicity).
+theorem MSCostBound (xs : List ℕ) (h : ∃ k, xs.length = 2 ^ k) :
+  (mergeSort xs).cost = xs.length*(Nat.log 2 xs.length)  := by
+  rw [mergeSort_cost_eq_MS_REC]
+  obtain ⟨k,hk⟩ := h
+  rw [hk,MS_REC_SIMP_EQ,MS_REC_SIMP_EQ_CLOSED]
+  simp only [Nat.lt_add_one, Nat.log_pow]
 
 end CostM
